wip

program_proof_rules.thy
@@ -15,6 +15,8 @@ thm execution_s_correct_def
  execution_s_correct ?progr ?S ?i \<equiv> \<forall>trace S'. ?S ~~ (?i, trace) \<leadsto>\<^sub>S* S' \<longrightarrow> traceCorrect_s ?progr trace
 *)
 
+find_consts "('a \<rightharpoonup> 'b) \<Rightarrow> ('a \<rightharpoonup> 'b) \<Rightarrow> ('a \<rightharpoonup> 'b)"
+
 definition execution_s_check where
   "execution_s_check 
   progr 
@@ -26,38 +28,60 @@ definition execution_s_check where
   s_knownIds 
   s_invocationOp
   s_invocationRes
+  generatedLocal
   vis
   tx
   ls
- \<equiv> s_invocationOp i \<noteq> None
-  \<and> (\<forall>trace S' x_ls x_cp x_vis x_txn x_txns x_gids. 
-      let S  = \<lparr>
-        calls = s_calls,
-        happensBefore = s_happensBefore,
-        callOrigin = s_callOrigin,
-        transactionOrigin = s_transactionOrigin,
-        knownIds = s_knownIds,
-        invocationOp = s_invocationOp,
-        invocationRes = s_invocationRes,
-        prog = progr,
-        transactionStatus = x_txns,
-        generatedIds = x_gids,
-        localState = x_ls(i \<mapsto> ls),
-        currentProc = x_cp(i \<mapsto> toImpl),
-        visibleCalls = x_vis(i \<mapsto> vis),
-        currentTransaction = x_txn(i := tx)
-      \<rparr>
-      in (S ~~ (i, trace) \<leadsto>\<^sub>S* S') \<longrightarrow> traceCorrect_s progr trace)"
+ \<equiv>  (\<forall>trace S1 S'. 
+           (S1 ~~ (i, trace) \<leadsto>\<^sub>S* S')
+       \<longrightarrow> (\<forall>p t. (AInvoc p, t) \<notin> set trace)
+       \<longrightarrow> state_wellFormed S1
+       \<longrightarrow> calls S1 = s_calls
+       \<longrightarrow> happensBefore S1 = s_happensBefore
+       \<longrightarrow> callOrigin S1 = s_callOrigin
+       \<longrightarrow> transactionOrigin S1 = s_transactionOrigin
+       \<longrightarrow> knownIds S1 = s_knownIds
+       \<longrightarrow> invocationOp S1 = s_invocationOp
+       \<longrightarrow> invocationRes S1 = s_invocationRes
+       \<longrightarrow> prog S1 = progr
+       \<longrightarrow> generatedLocal = {x. generatedIds S1 x \<triangleq> i}
+       \<longrightarrow> localState S1 i \<triangleq> ls
+       \<longrightarrow> currentProc S1 i \<triangleq> toImpl
+       \<longrightarrow> visibleCalls S1 i \<triangleq>  vis
+       \<longrightarrow> currentTransaction S1 i = tx
+       \<longrightarrow> traceCorrect_s  trace)"
+
+lemma beforeInvoc_execution_s_check: 
+  assumes "s_invocationOp i = None"
+  shows "
+execution_s_check   progr   i  s_calls   s_happensBefore   s_callOrigin   s_transactionOrigin   s_knownIds   s_invocationOp  s_invocationRes  generatedLocal  vis  tx  ls
+"
+  using assms  apply (auto simp add: execution_s_check_def)
+  apply (case_tac trace, auto)
+   apply (simp add: traceCorrect_s_def)
+  apply (auto simp add: steps_s_cons_simp Let_def)
+  find_theorems steps_s "(#)"
+  apply (erule step_s.cases, auto)
+  using wf_localState_to_invocationOp apply auto
+  by fastforce+
 
 
-text "It is sufficient to check with execution_s_check to ensure that the procedure is correct:"
+
+
+
+
+  text "It is sufficient to check with execution_s_check to ensure that the procedure is correct:"
+
+  find_theorems "\<lbrakk>?f ?x; ?x = ?y\<rbrakk> \<Longrightarrow> ?f ?y"
 
 lemma execution_s_check_sound:
-  assumes "localState S i \<triangleq> ls"
+  assumes  "localState S i \<triangleq> ls"
     and "visibleCalls S i \<triangleq> vis"
     and "localState S i \<triangleq> ls"
     and "prog S = progr"
     and "currentProc S i \<triangleq> toImpl"
+    and "generatedLocal = {x. generatedIds S x \<triangleq> i}"
+    and "state_wellFormed S"
     and c: "execution_s_check 
   progr 
   i
@@ -68,6 +92,7 @@ lemma execution_s_check_sound:
   (knownIds S)
   (invocationOp S)
   (invocationRes S)
+  generatedLocal
   vis
   (currentTransaction S i)
   ls"
@@ -76,19 +101,43 @@ proof (auto simp add:  execution_s_correct_def)
   fix trace S'
   assume a0: "S ~~ (i, trace) \<leadsto>\<^sub>S* S'"
 
-  from c
-  show "traceCorrect_s progr trace"
-    by (auto simp add: execution_s_check_def, 
-        smt a0 assms fun_upd_triv old.unit.exhaust state.surjective)
+
+  thm c[simplified execution_s_check_def]
+
+  from a0
+  show "traceCorrect_s  trace"
+  proof (rule c[simplified execution_s_check_def, rule_format]; force?)
+    show "state_wellFormed S"
+      by (simp add: assms(7))
+
+    show "\<And>p t. (AInvoc p, t) \<notin> set trace"
+      using a0 assms(1) assms(7) no_more_invoc by blast
+
+
+    show "prog S = progr"
+      by (simp add: assms(4))
+
+    show " generatedLocal = {x. generatedIds S x \<triangleq> i}"
+      by (auto simp add: assms(6))
+
+    show "localState S i \<triangleq> ls"
+      by (simp add: assms(1))
+
+    show "currentProc S i \<triangleq> toImpl"
+      by (simp add: assms(5))
+
+    show "visibleCalls S i \<triangleq> vis"
+      by (simp add: assms(2))
+  qed
 qed
 
-lemma traceCorrect_s_empty: "traceCorrect_s progr [] "
+lemma traceCorrect_s_empty: "traceCorrect_s  [] "
   by (simp add: traceCorrect_s_def) 
 
 lemma case_trace_not_empty:
-  assumes  "\<And>a trace'. trace = a#trace' \<Longrightarrow> traceCorrect_s progr (a#trace')"
-shows "traceCorrect_s progr trace"
-using assms by (cases trace, auto simp add: traceCorrect_s_empty)
+  assumes  "\<And>a trace'. trace = a#trace' \<Longrightarrow> traceCorrect_s  (a#trace')"
+  shows "traceCorrect_s  trace"
+  using assms by (cases trace, auto simp add: traceCorrect_s_empty)
 
 (*
 lemma proof_rule_soundness:
@@ -120,16 +169,44 @@ shows"execution_s_check
   (A \<bind> cont)
 "
 *)
-
-lemma 
-  assumes "\<not>finite (Collect P)"
-(* TODO add properties about uniqueness of v:
-  - not in calls
-  - not in ops/results
-  - not known
-  - not generated in current 
-*)
-and cont: "\<And>v. \<lbrakk>P v\<rbrakk> \<Longrightarrow> execution_s_check
+lemma execution_s_check_single_step:
+  assumes H: "\<And>S1 action Inv S'. \<lbrakk>
+  S1 ~~ (i,action,Inv) \<leadsto>\<^sub>S S';
+  invocationOp S1 i \<noteq> None;
+  calls S1 = s_calls;
+  happensBefore S1 = s_happensBefore;
+  callOrigin S1 = s_callOrigin;
+  transactionOrigin S1 = s_transactionOrigin;
+  knownIds S1 = s_knownIds;
+  invocationOp S1 = s_invocationOp;
+  invocationRes S1 = s_invocationRes;
+  prog S1 = progr;
+  generatedLocal = {x. generatedIds S1 x \<triangleq> i};
+  localState S1 i \<triangleq> ls;
+  currentProc S1 i \<triangleq> toImpl;
+  visibleCalls S1 i \<triangleq>  vis;
+  currentTransaction S1 i = tx
+\<rbrakk> \<Longrightarrow> 
+  Inv
+\<and> (case localState S' i of
+    None \<Rightarrow> True
+  | Some LS' \<Rightarrow>
+    execution_s_check
+    progr 
+    i
+    (calls S')
+    (happensBefore S')
+    (callOrigin S')
+    (transactionOrigin S')
+    (knownIds S')
+    (invocationOp S')
+    (invocationRes S')
+    {x. generatedIds S' x \<triangleq> i}
+    (case visibleCalls S' i of Some vis \<Rightarrow> vis | None \<Rightarrow> {})
+    (currentTransaction S' i)
+    LS')
+"
+shows"execution_s_check
   progr 
   i
   s_calls 
@@ -139,6 +216,199 @@ and cont: "\<And>v. \<lbrakk>P v\<rbrakk> \<Longrightarrow> execution_s_check
   s_knownIds 
   s_invocationOp
   s_invocationRes
+  generatedLocal
+  vis
+  tx
+  ls
+"
+proof (cases "s_invocationOp i")
+  case None
+  then show ?thesis
+    by (simp add: beforeInvoc_execution_s_check) 
+next
+  case (Some action)
+
+  show ?thesis
+  proof (auto simp add: execution_s_check_def)
+    fix trace S1 S'
+    assume a0: "S1 ~~ (i, trace) \<leadsto>\<^sub>S* S'"
+      and a1: "\<forall>p t. (AInvoc p, t) \<notin> set trace"
+      and a2: "state_wellFormed S1"
+      and a3: "s_calls = calls S1"
+      and a4: "s_happensBefore = happensBefore S1"
+      and a5: "s_callOrigin = callOrigin S1"
+      and a6: "s_transactionOrigin = transactionOrigin S1"
+      and a7: "s_knownIds = knownIds S1"
+      and a8: "s_invocationOp = invocationOp S1"
+      and a9: "s_invocationRes = invocationRes S1"
+      and a10: "progr = prog S1"
+      and a11: "generatedLocal = {x. generatedIds S1 x \<triangleq> i}"
+      and a12: "localState S1 i \<triangleq> ls"
+      and a13: "currentProc S1 i \<triangleq> toImpl"
+      and a14: "visibleCalls S1 i \<triangleq> vis"
+      and a15: "tx = currentTransaction S1 i"
+
+    show "traceCorrect_s  trace"
+    proof (cases trace)
+      case Nil
+      then show ?thesis
+        by (simp add: traceCorrect_s_empty) 
+
+    next
+      case (Cons a trace')
+      obtain action Inv where a_def[simp]: "a = (action, Inv)" by force
+
+      from `S1 ~~ (i, trace) \<leadsto>\<^sub>S* S'`
+      obtain S1'
+        where step: "S1 ~~ (i, action, Inv) \<leadsto>\<^sub>S S1'" 
+          and steps: "S1' ~~ (i, trace') \<leadsto>\<^sub>S* S'"
+          and trace_split: "trace = (action,Inv)#trace'"
+        using a_def local.Cons steps_s_cons_simp by blast
+
+
+      have gI: "\<forall>x\<in>generatedLocal. generatedIds S1 x \<triangleq> i"
+        using a11 by blast
+
+      have hasInvoc: "invocationOp S1 i \<noteq> None"
+        using Some a8 by auto
+
+
+      from step
+      have appliedH: "Inv \<and>
+    (case localState S1' i of None \<Rightarrow> True
+     | Some LS' \<Rightarrow>
+         execution_s_check progr i (calls S1') (happensBefore S1') (callOrigin S1') (transactionOrigin S1') (knownIds S1') (invocationOp S1')
+          (invocationRes S1') {x. generatedIds S1' x \<triangleq> i} (visibleCalls S1' i orElse {}) (currentTransaction S1' i) LS')"
+        by (rule H; (simp add: a3 a4 a5 a6 a7 a8 a9 a10 a11 a12 a13 a14 a15 hasInvoc))
+        
+
+
+      hence Inv
+        by simp
+
+      find_theorems "traceCorrect_s" "(#)"
+
+      show ?thesis
+        unfolding trace_split 
+      proof (rule traceCorrect_s_split; (simp add: `Inv`)?)
+
+        show "traceCorrect_s trace'"
+
+        proof (cases "localState S1' i")
+          case None
+
+          with steps have "trace' = []"
+            using local_state_None_no_more_steps
+            by (metis a0 a12 a2 insert_iff list.simps(15) local.Cons no_more_invoc option.simps(3)) 
+
+
+          then show ?thesis
+            using traceCorrect_s_empty by blast
+
+
+        next
+          case (Some LS')
+
+          with appliedH have "execution_s_check progr i (calls S1') (happensBefore S1') (callOrigin S1') (transactionOrigin S1') (knownIds S1') (invocationOp S1')
+          (invocationRes S1') {x. generatedIds S1' x \<triangleq> i} (visibleCalls S1' i orElse {}) (currentTransaction S1' i) LS'"
+            by auto
+
+          then
+          show ?thesis
+          proof (rule execution_s_check_def[THEN meta_eq_to_obj_eq, THEN iffD1, rule_format])
+            show "S1' ~~ (i, trace') \<leadsto>\<^sub>S* S'" using steps .
+            show "\<And>p t. (AInvoc p, t) \<notin> set trace'"
+              using Some a2 local.step no_more_invoc state_wellFormed_combine_s1 steps by fastforce
+            show "state_wellFormed S1'"
+              using a2 local.step state_wellFormed_combine_s1 by blast
+            show "prog S1' = progr"
+              by (metis a0 a10 steps unchangedProg)
+            show "localState S1' i \<triangleq> LS'"
+              by (simp add: Some)
+
+
+
+            show "currentProc S1' i \<triangleq> toImpl"
+              using step Some a13 by (auto simp add: step_s.simps a12 a2 wf_localState_to_invocationOp)
+
+            show "visibleCalls S1' i \<triangleq> visibleCalls S1' i orElse {}"
+              using step a14 Some  by (auto simp add: step_s.simps a12 a2 wf_localState_to_invocationOp split: option.splits)
+
+          qed auto
+        qed
+      qed
+    qed
+  qed
+qed
+
+lemma back_subst2: "\<lbrakk>P x'1 x'2; x'1 = x1; x'2 = x2 \<rbrakk> \<Longrightarrow>  P x1 x2" by auto 
+lemma back_subst3: "\<lbrakk>P x'1 x'2 x'3; x'1 = x1; x'2 = x2; x'3 = x3 \<rbrakk> \<Longrightarrow>  P x1 x2 x3" by auto 
+lemma back_subst4: "\<lbrakk>P x'1 x'2 x'3 x'4; x'1 = x1; x'2 = x2; x'3 = x3; x'4 = x4 \<rbrakk> \<Longrightarrow>  P x1 x2 x3 x4" by auto 
+lemma back_subst5: "\<lbrakk>P x'1 x'2 x'3 x'4 x'5; x'1 = x1; x'2 = x2; x'3 = x3; x'4 = x4; x'5 = x5 \<rbrakk> \<Longrightarrow>  P x1 x2 x3 x4 x5" by auto 
+lemma back_subst6: "\<lbrakk>P x'1 x'2 x'3 x'4 x'5 x'6; x'1 = x1; x'2 = x2; x'3 = x3; x'4 = x4; x'5 = x5; x'6 = x6 \<rbrakk> \<Longrightarrow>  P x1 x2 x3 x4 x5 x6" by auto 
+lemma back_subst7: "\<lbrakk>P x'1 x'2 x'3 x'4 x'5 x'6 x'7; x'1 = x1; x'2 = x2; x'3 = x3; x'4 = x4; x'5 = x5; x'6 = x6; x'7 = x7 \<rbrakk> \<Longrightarrow>  P x1 x2 x3 x4 x5 x6 x7" by auto 
+lemma back_subst8: "\<lbrakk>P x'1 x'2 x'3 x'4 x'5 x'6 x'7 x'8; x'1 = x1; x'2 = x2; x'3 = x3; x'4 = x4; x'5 = x5; x'6 = x6; x'7 = x7; x'8 = x8 \<rbrakk> \<Longrightarrow>  P x1 x2 x3 x4 x5 x6 x7 x8" by auto 
+lemma back_subst9: "\<lbrakk>P x'1 x'2 x'3 x'4 x'5 x'6 x'7 x'8 x'9; x'1 = x1; x'2 = x2; x'3 = x3; x'4 = x4; x'5 = x5; x'6 = x6; x'7 = x7; x'8 = x8; x'9 = x9 \<rbrakk> \<Longrightarrow>  P x1 x2 x3 x4 x5 x6 x7 x8 x9" by auto 
+lemma back_subst10: "\<lbrakk>P x'1 x'2 x'3 x'4 x'5 x'6 x'7 x'8 x'9 x'10; x'1 = x1; x'2 = x2; x'3 = x3; x'4 = x4; x'5 = x5; x'6 = x6; x'7 = x7; x'8 = x8; x'9 = x9; x'10 = x10 \<rbrakk> \<Longrightarrow>  P x1 x2 x3 x4 x5 x6 x7 x8 x9 x10" by auto 
+lemma back_subst11: "\<lbrakk>P x'1 x'2 x'3 x'4 x'5 x'6 x'7 x'8 x'9 x'10 x'11; x'1 = x1; x'2 = x2; x'3 = x3; x'4 = x4; x'5 = x5; x'6 = x6; x'7 = x7; x'8 = x8; x'9 = x9; x'10 = x10; x'11 = x11 \<rbrakk> \<Longrightarrow>  P x1 x2 x3 x4 x5 x6 x7 x8 x9 x10 x11" by auto 
+lemma back_subst12: "\<lbrakk>P x'1 x'2 x'3 x'4 x'5 x'6 x'7 x'8 x'9 x'10 x'11 x'12; x'1 = x1; x'2 = x2; x'3 = x3; x'4 = x4; x'5 = x5; x'6 = x6; x'7 = x7; x'8 = x8; x'9 = x9; x'10 = x10; x'11 = x11; x'12 = x12 \<rbrakk> \<Longrightarrow>  P x1 x2 x3 x4 x5 x6 x7 x8 x9 x10 x11 x12" by auto 
+lemma back_subst13: "\<lbrakk>P x'1 x'2 x'3 x'4 x'5 x'6 x'7 x'8 x'9 x'10 x'11 x'12 x'13; x'1 = x1; x'2 = x2; x'3 = x3; x'4 = x4; x'5 = x5; x'6 = x6; x'7 = x7; x'8 = x8; x'9 = x9; x'10 = x10; x'11 = x11; x'12 = x12; x'13 = x13 \<rbrakk> \<Longrightarrow>  P x1 x2 x3 x4 x5 x6 x7 x8 x9 x10 x11 x12 x13" by auto 
+lemma back_subst14: "\<lbrakk>P x'1 x'2 x'3 x'4 x'5 x'6 x'7 x'8 x'9 x'10 x'11 x'12 x'13 x'14; x'1 = x1; x'2 = x2; x'3 = x3; x'4 = x4; x'5 = x5; x'6 = x6; x'7 = x7; x'8 = x8; x'9 = x9; x'10 = x10; x'11 = x11; x'12 = x12; x'13 = x13; x'14 = x14 \<rbrakk> \<Longrightarrow>  P x1 x2 x3 x4 x5 x6 x7 x8 x9 x10 x11 x12 x13 x14" by auto 
+lemma back_subst15: "\<lbrakk>P x'1 x'2 x'3 x'4 x'5 x'6 x'7 x'8 x'9 x'10 x'11 x'12 x'13 x'14 x'15; x'1 = x1; x'2 = x2; x'3 = x3; x'4 = x4; x'5 = x5; x'6 = x6; x'7 = x7; x'8 = x8; x'9 = x9; x'10 = x10; x'11 = x11; x'12 = x12; x'13 = x13; x'14 = x14; x'15 = x15 \<rbrakk> \<Longrightarrow>  P x1 x2 x3 x4 x5 x6 x7 x8 x9 x10 x11 x12 x13 x14 x15" by auto 
+lemma back_subst16: "\<lbrakk>P x'1 x'2 x'3 x'4 x'5 x'6 x'7 x'8 x'9 x'10 x'11 x'12 x'13 x'14 x'15 x'16; x'1 = x1; x'2 = x2; x'3 = x3; x'4 = x4; x'5 = x5; x'6 = x6; x'7 = x7; x'8 = x8; x'9 = x9; x'10 = x10; x'11 = x11; x'12 = x12; x'13 = x13; x'14 = x14; x'15 = x15; x'16 = x16 \<rbrakk> \<Longrightarrow>  P x1 x2 x3 x4 x5 x6 x7 x8 x9 x10 x11 x12 x13 x14 x15 x16" by auto 
+lemma back_subst17: "\<lbrakk>P x'1 x'2 x'3 x'4 x'5 x'6 x'7 x'8 x'9 x'10 x'11 x'12 x'13 x'14 x'15 x'16 x'17; x'1 = x1; x'2 = x2; x'3 = x3; x'4 = x4; x'5 = x5; x'6 = x6; x'7 = x7; x'8 = x8; x'9 = x9; x'10 = x10; x'11 = x11; x'12 = x12; x'13 = x13; x'14 = x14; x'15 = x15; x'16 = x16; x'17 = x17 \<rbrakk> \<Longrightarrow>  P x1 x2 x3 x4 x5 x6 x7 x8 x9 x10 x11 x12 x13 x14 x15 x16 x17" by auto 
+lemma back_subst18: "\<lbrakk>P x'1 x'2 x'3 x'4 x'5 x'6 x'7 x'8 x'9 x'10 x'11 x'12 x'13 x'14 x'15 x'16 x'17 x'18; x'1 = x1; x'2 = x2; x'3 = x3; x'4 = x4; x'5 = x5; x'6 = x6; x'7 = x7; x'8 = x8; x'9 = x9; x'10 = x10; x'11 = x11; x'12 = x12; x'13 = x13; x'14 = x14; x'15 = x15; x'16 = x16; x'17 = x17; x'18 = x18 \<rbrakk> \<Longrightarrow>  P x1 x2 x3 x4 x5 x6 x7 x8 x9 x10 x11 x12 x13 x14 x15 x16 x17 x18" by auto 
+lemma back_subst19: "\<lbrakk>P x'1 x'2 x'3 x'4 x'5 x'6 x'7 x'8 x'9 x'10 x'11 x'12 x'13 x'14 x'15 x'16 x'17 x'18 x'19; x'1 = x1; x'2 = x2; x'3 = x3; x'4 = x4; x'5 = x5; x'6 = x6; x'7 = x7; x'8 = x8; x'9 = x9; x'10 = x10; x'11 = x11; x'12 = x12; x'13 = x13; x'14 = x14; x'15 = x15; x'16 = x16; x'17 = x17; x'18 = x18; x'19 = x19 \<rbrakk> \<Longrightarrow>  P x1 x2 x3 x4 x5 x6 x7 x8 x9 x10 x11 x12 x13 x14 x15 x16 x17 x18 x19" by auto 
+lemma back_subst20: "\<lbrakk>P x'1 x'2 x'3 x'4 x'5 x'6 x'7 x'8 x'9 x'10 x'11 x'12 x'13 x'14 x'15 x'16 x'17 x'18 x'19 x'20; x'1 = x1; x'2 = x2; x'3 = x3; x'4 = x4; x'5 = x5; x'6 = x6; x'7 = x7; x'8 = x8; x'9 = x9; x'10 = x10; x'11 = x11; x'12 = x12; x'13 = x13; x'14 = x14; x'15 = x15; x'16 = x16; x'17 = x17; x'18 = x18; x'19 = x19; x'20 = x20 \<rbrakk> \<Longrightarrow>  P x1 x2 x3 x4 x5 x6 x7 x8 x9 x10 x11 x12 x13 x14 x15 x16 x17 x18 x19 x20" by auto 
+
+method back_subst for P :: "'a1 \<Rightarrow> bool" uses rule = (rule back_subst[where P=P], rule rule)
+ method back_subst2 for P :: "'a1\<Rightarrow>'a2 \<Rightarrow> bool" uses rule = (rule back_subst2[where P=P], rule rule) 
+ method back_subst3 for P :: "'a1\<Rightarrow>'a2\<Rightarrow>'a3 \<Rightarrow> bool" uses rule = (rule back_subst3[where P=P], rule rule) 
+ method back_subst4 for P :: "'a1\<Rightarrow>'a2\<Rightarrow>'a3\<Rightarrow>'a4 \<Rightarrow> bool" uses rule = (rule back_subst4[where P=P], rule rule) 
+ method back_subst5 for P :: "'a1\<Rightarrow>'a2\<Rightarrow>'a3\<Rightarrow>'a4\<Rightarrow>'a5 \<Rightarrow> bool" uses rule = (rule back_subst5[where P=P], rule rule) 
+ method back_subst6 for P :: "'a1\<Rightarrow>'a2\<Rightarrow>'a3\<Rightarrow>'a4\<Rightarrow>'a5\<Rightarrow>'a6 \<Rightarrow> bool" uses rule = (rule back_subst6[where P=P], rule rule) 
+ method back_subst7 for P :: "'a1\<Rightarrow>'a2\<Rightarrow>'a3\<Rightarrow>'a4\<Rightarrow>'a5\<Rightarrow>'a6\<Rightarrow>'a7 \<Rightarrow> bool" uses rule = (rule back_subst7[where P=P], rule rule) 
+ method back_subst8 for P :: "'a1\<Rightarrow>'a2\<Rightarrow>'a3\<Rightarrow>'a4\<Rightarrow>'a5\<Rightarrow>'a6\<Rightarrow>'a7\<Rightarrow>'a8 \<Rightarrow> bool" uses rule = (rule back_subst8[where P=P], rule rule) 
+ method back_subst9 for P :: "'a1\<Rightarrow>'a2\<Rightarrow>'a3\<Rightarrow>'a4\<Rightarrow>'a5\<Rightarrow>'a6\<Rightarrow>'a7\<Rightarrow>'a8\<Rightarrow>'a9 \<Rightarrow> bool" uses rule = (rule back_subst9[where P=P], rule rule) 
+ method back_subst10 for P :: "'a1\<Rightarrow>'a2\<Rightarrow>'a3\<Rightarrow>'a4\<Rightarrow>'a5\<Rightarrow>'a6\<Rightarrow>'a7\<Rightarrow>'a8\<Rightarrow>'a9\<Rightarrow>'a10 \<Rightarrow> bool" uses rule = (rule back_subst10[where P=P], rule rule) 
+ method back_subst11 for P :: "'a1\<Rightarrow>'a2\<Rightarrow>'a3\<Rightarrow>'a4\<Rightarrow>'a5\<Rightarrow>'a6\<Rightarrow>'a7\<Rightarrow>'a8\<Rightarrow>'a9\<Rightarrow>'a10\<Rightarrow>'a11 \<Rightarrow> bool" uses rule = (rule back_subst11[where P=P], rule rule) 
+ method back_subst12 for P :: "'a1\<Rightarrow>'a2\<Rightarrow>'a3\<Rightarrow>'a4\<Rightarrow>'a5\<Rightarrow>'a6\<Rightarrow>'a7\<Rightarrow>'a8\<Rightarrow>'a9\<Rightarrow>'a10\<Rightarrow>'a11\<Rightarrow>'a12 \<Rightarrow> bool" uses rule = (rule back_subst12[where P=P], rule rule) 
+ method back_subst13 for P :: "'a1\<Rightarrow>'a2\<Rightarrow>'a3\<Rightarrow>'a4\<Rightarrow>'a5\<Rightarrow>'a6\<Rightarrow>'a7\<Rightarrow>'a8\<Rightarrow>'a9\<Rightarrow>'a10\<Rightarrow>'a11\<Rightarrow>'a12\<Rightarrow>'a13 \<Rightarrow> bool" uses rule = (rule back_subst13[where P=P], rule rule) 
+ method back_subst14 for P :: "'a1\<Rightarrow>'a2\<Rightarrow>'a3\<Rightarrow>'a4\<Rightarrow>'a5\<Rightarrow>'a6\<Rightarrow>'a7\<Rightarrow>'a8\<Rightarrow>'a9\<Rightarrow>'a10\<Rightarrow>'a11\<Rightarrow>'a12\<Rightarrow>'a13\<Rightarrow>'a14 \<Rightarrow> bool" uses rule = (rule back_subst14[where P=P], rule rule) 
+ method back_subst15 for P :: "'a1\<Rightarrow>'a2\<Rightarrow>'a3\<Rightarrow>'a4\<Rightarrow>'a5\<Rightarrow>'a6\<Rightarrow>'a7\<Rightarrow>'a8\<Rightarrow>'a9\<Rightarrow>'a10\<Rightarrow>'a11\<Rightarrow>'a12\<Rightarrow>'a13\<Rightarrow>'a14\<Rightarrow>'a15 \<Rightarrow> bool" uses rule = (rule back_subst15[where P=P], rule rule) 
+ method back_subst16 for P :: "'a1\<Rightarrow>'a2\<Rightarrow>'a3\<Rightarrow>'a4\<Rightarrow>'a5\<Rightarrow>'a6\<Rightarrow>'a7\<Rightarrow>'a8\<Rightarrow>'a9\<Rightarrow>'a10\<Rightarrow>'a11\<Rightarrow>'a12\<Rightarrow>'a13\<Rightarrow>'a14\<Rightarrow>'a15\<Rightarrow>'a16 \<Rightarrow> bool" uses rule = (rule back_subst16[where P=P], rule rule) 
+ method back_subst17 for P :: "'a1\<Rightarrow>'a2\<Rightarrow>'a3\<Rightarrow>'a4\<Rightarrow>'a5\<Rightarrow>'a6\<Rightarrow>'a7\<Rightarrow>'a8\<Rightarrow>'a9\<Rightarrow>'a10\<Rightarrow>'a11\<Rightarrow>'a12\<Rightarrow>'a13\<Rightarrow>'a14\<Rightarrow>'a15\<Rightarrow>'a16\<Rightarrow>'a17 \<Rightarrow> bool" uses rule = (rule back_subst17[where P=P], rule rule) 
+ method back_subst18 for P :: "'a1\<Rightarrow>'a2\<Rightarrow>'a3\<Rightarrow>'a4\<Rightarrow>'a5\<Rightarrow>'a6\<Rightarrow>'a7\<Rightarrow>'a8\<Rightarrow>'a9\<Rightarrow>'a10\<Rightarrow>'a11\<Rightarrow>'a12\<Rightarrow>'a13\<Rightarrow>'a14\<Rightarrow>'a15\<Rightarrow>'a16\<Rightarrow>'a17\<Rightarrow>'a18 \<Rightarrow> bool" uses rule = (rule back_subst18[where P=P], rule rule) 
+ method back_subst19 for P :: "'a1\<Rightarrow>'a2\<Rightarrow>'a3\<Rightarrow>'a4\<Rightarrow>'a5\<Rightarrow>'a6\<Rightarrow>'a7\<Rightarrow>'a8\<Rightarrow>'a9\<Rightarrow>'a10\<Rightarrow>'a11\<Rightarrow>'a12\<Rightarrow>'a13\<Rightarrow>'a14\<Rightarrow>'a15\<Rightarrow>'a16\<Rightarrow>'a17\<Rightarrow>'a18\<Rightarrow>'a19 \<Rightarrow> bool" uses rule = (rule back_subst19[where P=P], rule rule) 
+ method back_subst20 for P :: "'a1\<Rightarrow>'a2\<Rightarrow>'a3\<Rightarrow>'a4\<Rightarrow>'a5\<Rightarrow>'a6\<Rightarrow>'a7\<Rightarrow>'a8\<Rightarrow>'a9\<Rightarrow>'a10\<Rightarrow>'a11\<Rightarrow>'a12\<Rightarrow>'a13\<Rightarrow>'a14\<Rightarrow>'a15\<Rightarrow>'a16\<Rightarrow>'a17\<Rightarrow>'a18\<Rightarrow>'a19\<Rightarrow>'a20 \<Rightarrow> bool" uses rule = (rule back_subst20[where P=P], rule rule) 
+
+
+lemma execution_s_check_newId:
+  assumes "infinite (Collect P)"
+    (* TODO add properties about uniqueness of v:
+  - not in calls
+  - not in ops/results
+  - not known
+  - not generated in current 
+*)
+    and cont: "\<And>v. \<lbrakk>P v; 
+ new_unique_not_in_calls s_calls v;
+new_unique_not_in_invocationOp v;
+new_unique_not_in_invocationRes v;
+new_unique_not_in_knownIds v;
+new_unique_not_generated_in_current v;
+uniqueIds v = {to_nat v}
+\<rbrakk> \<Longrightarrow> execution_s_check
+  progr 
+  i
+  s_calls 
+  s_happensBefore 
+  s_callOrigin 
+  s_transactionOrigin 
+  s_knownIds 
+  s_invocationOp
+  s_invocationRes
+  (localGenerated \<union> {to_nat v})
   vis
   tx
   (cont v)"
@@ -153,36 +423,34 @@ shows"execution_s_check
   s_knownIds 
   s_invocationOp
   s_invocationRes
+  localGenerated
   vis
   tx
   (newId P \<bind> cont)
 "
-proof -
+proof (rule  execution_s_check_single_step, auto simp add: step_s.simps split: if_splits, goal_cases "goal")
+  case (goal S1 Inv y uidv)
+  show ?case 
+  proof (rule back_subst13[where P=execution_s_check], rule cont; (simp add: goal; fail)?)
+    show "localGenerated \<union> {to_nat uidv} = {x. x \<noteq> to_nat uidv \<longrightarrow> generatedIds S1 x \<triangleq> i}"
+      using `localGenerated = {x. generatedIds S1 x \<triangleq> i}` by auto
 
-  obtain v where "P v"
-    using assms(1) infinite_imp_nonempty by auto
+      show "new_unique_not_in_invocationOp uidv"
+        sorry
+      show "new_unique_not_in_invocationRes uidv"
+        sorry
+      show "new_unique_not_in_knownIds uidv"
+        sorry
+      show "new_unique_not_generated_in_current uidv"
+        sorry
+      show " new_unique_not_in_calls s_calls uidv"
+        sorry
+    qed
+  qed
 
-  from this and cont 
-  have "execution_s_check progr i s_calls s_happensBefore s_callOrigin s_transactionOrigin s_knownIds s_invocationOp s_invocationRes vis tx   (cont v)"
-    by blast
 
 
-  from this
-  obtain currentInvocationOp 
-    where [simp]: "s_invocationOp i \<triangleq> currentInvocationOp"
-    by (auto simp add: execution_s_check_def)
 
-  show ?thesis
-
-    apply (auto simp add: execution_s_check_def)
-
-    apply (rule case_trace_not_empty)
-    apply (auto simp add: steps_s_cons_simp)
-    apply (erule step_s.cases)
-          apply (auto split: if_splits)
-    apply (smt Pair_inject cont execution_s_check_def insert_iff list.simps(15) traceCorrect_s_def)
-    done
-qed
 
 
 
