example_userbase.thy
@@ -270,6 +270,30 @@ proof (auto simp add: program_wellFormed_def)
 qed
 
 
+lemma no_more_invoc:
+  assumes steps: "S ~~ (i, trace) \<leadsto>\<^sub>S* S'"
+and ls: "localState S i \<noteq> None"
+and wf: "state_wellFormed S"
+shows "(AInvoc p, t) \<notin> set trace"
+proof -
+
+  from ls have no_invoc: "invocationOp S (fst (i, trace)) \<noteq> None"
+    by (simp add: wf wf_localState_to_invocationOp)
+
+
+  have "(AInvoc p, t) \<notin> set (snd (i, trace))"
+  using steps no_invoc
+proof (induct rule: steps_s.induct)
+case (steps_s_refl S s)
+  then show ?case 
+    by auto
+
+next
+  case (steps_s_step S s tr S' a S'')
+  then show ?case 
+    by (auto simp add: step_s.simps has_invocationOp_forever)
+qed
+
 
 lemma invariant_progr[simp]: "invariant progr = example_userbase.inv"
       by (auto simp add: progr_def)
