repliss_sem_single_invocation.thy
@@ -404,6 +404,13 @@ inductive steps_s :: "('proc::valueType, 'ls, 'operation, 'any::valueType) state
 definition traceCorrect_s where
 "traceCorrect_s program trace \<equiv> (\<forall>a. (a, False) \<notin> set trace)"
 
+lemma traceCorrect_s_split: 
+  assumes "snd a"
+and "traceCorrect_s progr trace"
+shows "traceCorrect_s progr (a#trace)"
+  by (metis assms set_ConsD sndI traceCorrect_s_def)
+
+
 definition programCorrect_s where
 "programCorrect_s program \<equiv> (\<forall>trace s S. 
    (initialState program ~~ (s, trace) \<leadsto>\<^sub>S* S)
