single_invocation_correctness2.thy
@@ -171,6 +171,44 @@ qed
 
 
 
+lemma no_more_invoc:
+  assumes steps: "S ~~ (i, trace) \<leadsto>\<^sub>S* S'"
+    and ls: "localState S i \<noteq> None"
+    and wf: "state_wellFormed S"
+  shows "(AInvoc p, t) \<notin> set trace"
+proof -
+
+  from ls have no_invoc: "invocationOp S (fst (i, trace)) \<noteq> None"
+    by (simp add: wf wf_localState_to_invocationOp)
+
+
+  have "(AInvoc p, t) \<notin> set (snd (i, trace))"
+    using steps no_invoc
+  proof (induct rule: steps_s.induct)
+    case (steps_s_refl S s)
+    then show ?case 
+      by auto
+
+  next
+    case (steps_s_step S s tr S' a S'')
+    then show ?case 
+      by (auto simp add: step_s.simps has_invocationOp_forever)
+  qed
+  thus ?thesis
+    by auto
+qed
+
+lemma local_state_None_no_more_steps:
+assumes steps: "S ~~ (i, trace) \<leadsto>\<^sub>S* S'"
+and "localState S i = None"
+and "\<And>p t. (AInvoc p, t) \<notin> set trace"
+shows "trace = []"
+proof -
+  have "snd (i,trace) = []" if  "localState S (fst (i,trace)) = None" and "\<And>p t. (AInvoc p, t) \<notin> set (snd (i,trace))"
+    using steps that by (induct, auto simp add: step_s.simps steps_s_empty)
+  thus ?thesis
+    using assms by auto
+qed
 
 
 end
